finished elaborating the Fixed Payout contract

FixedPayout/FixedPayout.fst
@@ -20,14 +20,24 @@ module Str   = FStar.String
 module CId   = Zen.ContractId
 module SMT   = Zen.SparseMerkleTree
 
-type ticker = s:string {Str.length s <= 4}
+type parser (a:Type) (m:nat) =
+    option (Dict.t data) -> result a `cost` m
+
+type hashUpdate (a:Type) (m:nat) =
+    a -> Sha3.t -> Sha3.t `cost` m
+
+type ticker =
+    s:string { Str.length s <= 4 }
 
 // compressed public key
-type cpk = byte ** hash
+type cpk =
+    byte ** hash
 
-type preAuditPath = p: list data{length p == 256}
+type preAuditPath =
+    p: list data { length p == 256 }
 
-type auditPath = p: list hash{length p == 256}
+type auditPath =
+    p: list hash { length p == 256 }
 
 type attestation = {
     timestamp  : timestamp;
@@ -81,9 +91,9 @@ type redemption = {
 // if all of the mappings return Some, then returns Some list.
 // otherwise returns None.
 val tryMap(#a #b: Type)(#n: nat):
-  (a -> option b `cost` n)
-  -> ls:list a
-  -> option (ls':list b{length ls' == length ls}) `cost` (length ls * n)
+    (a -> option b `cost` n)
+    -> ls:list a
+    -> option (ls':list b{length ls' == length ls}) `cost` (length ls * (n + 20) + 20)
 let rec tryMap #a #b #n f ls = //20
     match ls with
     | hd::tl ->
@@ -93,49 +103,53 @@ let rec tryMap #a #b #n f ls = //20
         | Some hd', Some tl' ->
             let (result: list b{length result == length ls}) = hd'::tl' in
             OptT.some result
-        | _ -> OptT.none
-        end
-    | [] -> [] |> OptT.incSome (length ls * n)
+        | _ -> OptT.none end
+    | [] -> [] |> OptT.incSome (length ls * (n + 20))
 
-let runOpt (#a #s:Type) (#m:nat) (update:a -> s -> s `cost` m) (x:option a) (st:s): s `cost` m =
+
+let runOpt (#a #s:Type) (#m:nat) (update:a -> s -> s `cost` m) (x:option a) (st:s): s `cost` (m + 5) =
     Opt.maybe (incRet m) update x st
 
 // compress a public key
-let compress (pk:publicKey): cpk `cost` 132 =
+let compress (pk:publicKey): cpk `cost` 305 = // 13
     let open U8 in
-    let parity = (Array.item 32 pk %^ 2uy) +^ 2uy in
-    let aux (i:nat{i < 32}): byte `cost` 0 =
-        ret (Array.item (31-i) pk) in
-    let! x = Array.init_pure 32 aux in
+    let aux (i : nat { i < 32 }) : byte `cost` 5 =
+        ret (Array.item (31 - i) pk)
+    in
+    let  parity = (Array.item 32 pk %^ 2uy) +^ 2uy in
+    let! x      = Array.init_pure 32 aux           in // 292
     ret (parity, x)
 
-let updateCPK ((parity, h):cpk) (s:Sha3.t): Sha3.t `cost` 198 =
+let updateCPK ((parity, h):cpk) (s:Sha3.t): Sha3.t `cost` 205 = // 7
     ret s
-    >>= Sha3.updateByte parity
-    >>= Sha3.updateHash h
+    >>= Sha3.updateByte parity // 6
+    >>= Sha3.updateHash h // 192
 
 // hash a compressed publicKey
-let hashCPK (cpk:cpk): hash `cost` 218 =
+let hashCPK (cpk:cpk): hash `cost` 231 = // 6
     ret Sha3.empty
-    >>= updateCPK cpk
-    >>= Sha3.finalize
+    >>= updateCPK cpk // 205
+    >>= Sha3.finalize // 20
 
-val lockToPubKey: asset -> U64.t -> publicKey -> txSkeleton -> txSkeleton `cost` 414
-let lockToPubKey asset amount pk tx =
-    let! cpk = compress pk in
-    let! cpkHash = hashCPK cpk in
-    TX.lockToPubKey asset amount cpkHash tx
+val lockToPubKey: asset -> U64.t -> publicKey -> txSkeleton -> txSkeleton `cost` 610
+let lockToPubKey asset amount pk tx = // 10
+    let! cpk     = compress pk in // 305
+    let! cpkHash = hashCPK cpk in // 231
+    TX.lockToPubKey asset amount cpkHash tx // 64
 
-val lockToSender: asset -> U64.t -> sender -> txSkeleton -> txSkeleton `cost` 414
-let lockToSender asset amount sender =
+val lockToSender: asset -> U64.t -> sender -> txSkeleton -> txSkeleton `cost` 623
+let lockToSender asset amount sender txSkel = // 13
     match sender with
     | PK pk ->
-        lockToPubKey asset amount pk
+        txSkel
+        |> lockToPubKey asset amount pk // 610
     | Contract cid ->
-        TX.lockToContract asset amount cid
-        >> inc 350
+        txSkel
+        |> TX.lockToContract asset amount cid // 64
+        |> inc 546
     | Anonymous ->
-        incRet 414
+        txSkel
+        |> incRet 610
 
 
 
@@ -145,12 +159,12 @@ let lockToSender asset amount sender =
 -------------------------------------------------------------------------------
 *)
 
-val parseDict: option data -> result (option (Dict.t data)) `cost` 4
-let parseDict data =
+val parseDict: option data -> result (option (Dict.t data)) `cost` 15
+let parseDict data = // 11
     match data with
     | Some data ->
         data
-        |> tryDict
+        |> tryDict // 4
         |> RT.ofOptionT "Data parsing failed - the message body isn't a dictionary"
         |> RT.map Some
     | None ->
@@ -161,9 +175,9 @@ val parseField (#a:Type) (#m:nat)
     -> fieldName:string
     -> errMsg:string
     -> option (Dict.t data)
-    -> result a `cost` (m + 64)
-let parseField #_ #_ parser fieldName errMsg dict =
-    let! value = dict >!= Dict.tryFind fieldName >?= parser in
+    -> result a `cost` (m + 75)
+let parseField #_ #_ parser fieldName errMsg dict = // 11
+    let! value = dict >!= Dict.tryFind fieldName >?= parser in // (m + 64)
     match value with
     | Some value ->
         RT.ok value
@@ -174,99 +188,129 @@ val parseOptField (#a:Type) (#m:nat)
     : (data -> option a `cost` m)
     -> fieldName:string
     -> option (Dict.t data)
-    -> result (option a) `cost` (m + 64)
-let parseOptField #_ #_ parser fieldName dict =
+    -> result (option a) `cost` (m + 71)
+let parseOptField #_ #_ parser fieldName dict = // 7
     dict
-    >!= Dict.tryFind fieldName
-    >?= parser
+    >!= Dict.tryFind fieldName // 64
+    >?= parser // m
     >>= RT.ok
 
-val parseTicker: string -> string -> option (Dict.t data) -> result ticker `cost` 66
-let parseTicker fieldName errMsg dict =
+val parseTicker: string -> string -> option (Dict.t data) -> result ticker `cost` 90
+let parseTicker fieldName errMsg dict = // 6
     let open RT in
-    parseField tryString fieldName errMsg dict >>=
-    begin fun s ->
+    parseField tryString fieldName errMsg dict >>= // 77
+    begin fun s -> // 7
         if Str.length s <= 4
             then RT.ok (s <: ticker)
             else RT.failw "Ticker size can't be bigger than 4"
     end
 
-val extractHashes: string -> ls:list data -> result (ls':list hash {length ls' == length ls}) `cost` (length ls * 2)
-let extractHashes errMsg ls =
-    tryMap tryHash ls
+//val extractHashes: string -> ls:list data -> result (ls':list hash { length ls' == length ls }) `cost` (length ls * 22 + 25)
+let extractHashes errMsg ls = // 5
+    tryMap tryHash ls // (length ls * 22 + 20)
     |> RT.ofOptionT errMsg
 
-val extractAuditPath: preAuditPath -> result auditPath `cost` 512
-let extractAuditPath ls =
+val extractAuditPath: preAuditPath -> result auditPath `cost` 5661
+let extractAuditPath ls = // 4
     let open RT in
-    extractHashes "All the items in the audit path must be hashes" ls
-    $> (fun xs -> let (xs:list hash {length xs == 256}) = xs in xs)
+    extractHashes "All the items in the audit path must be hashes" ls // 5657 = 256 * 22 + 25
+    $> (fun xs -> let (xs:list hash { length xs == 256 }) = xs in xs)
 
-val parsePreAuditPath: string -> string -> option (Dict.t data) -> result preAuditPath `cost` 68
-let parsePreAuditPath fieldName errMsg dict =
+val parsePreAuditPath: string -> string -> option (Dict.t data) -> result preAuditPath `cost` 92
+let parsePreAuditPath fieldName errMsg dict = // 6
     let open RT in
-    parseField tryList fieldName errMsg dict >>=
-    begin fun ls ->
+    parseField tryList fieldName errMsg dict >>= // 79
+    begin fun ls -> // 7
         if length ls = 256
             then RT.ok (ls <: preAuditPath)
             else RT.failw "AuditPath length must be 256"
     end
 
-val parseAuditPath: string -> string -> option (Dict.t data) -> result auditPath `cost` 580
-let parseAuditPath fieldName errMsg =
+val parseAuditPath: string -> string -> option (Dict.t data) -> result auditPath `cost` 5760
+let parseAuditPath fieldName errMsg dict = // 7
     let open RT in
-    parsePreAuditPath fieldName errMsg
-    >=> extractAuditPath
+    ret dict
+    >>= parsePreAuditPath fieldName errMsg // 92
+    >>= extractAuditPath // 5661
 
-val parsePosition: string -> string -> option (Dict.t data) -> result position `cost` 66
-let parsePosition fieldName errMsg dict =
+val parsePosition: string -> string -> option (Dict.t data) -> result position `cost` 87
+let parsePosition fieldName errMsg dict = // 6
     let open RT in
-    parseField tryString fieldName errMsg dict >>=
-    begin function
+    parseField tryString fieldName errMsg dict >>= // 77
+    begin fun s -> match s with // 4
     | "Bull" -> ret Bull
     | "Bear" -> ret Bear
     | _      -> RT.failw "Position must be either Bull or Bear"
     end
 
-val parseContractId: string -> string -> option (Dict.t data) -> result contractId `cost` 130
-let parseContractId fieldName errMsg dict =
+val parseContractId: string -> string -> option (Dict.t data) -> result contractId `cost` 158
+let parseContractId fieldName errMsg dict = // 6
     let open RT in
-    parseField tryString fieldName errMsg dict >>=
-    begin fun s ->
+    parseField tryString fieldName errMsg dict >>= // 77
+    begin fun s -> // 11
         if Str.length s = 72
             then
                 let (s:string { Str.length s = 72 }) = s in
                 s
-                |> CId.parse
+                |> CId.parse // 64
                 |> RT.ofOptionT "The given OracleContractId is not a valid contractId"
             else
                 RT.incFailw 64 "OracleContractId must be 72 characters long"
     end
 
-let getTimestamp        = parseField      tryU64       "Timestamp"        "Could not parse Timestamp"
-let getCommit           = parseField      tryHash      "Commit"           "Could not parse Commit"
-let getOraclePubKey     = parseField      tryPublicKey "OraclePubKey"     "Could not parse OraclePubKey"
-let getTicker           = parseTicker                  "Ticker"           "Could not parse Ticker"
-let getPriceLow         = parseField      tryU64       "PriceLow"         "Could not parse PriceLow"
-let getPriceHigh        = parseOptField   tryU64       "PriceHigh"
-let getTimeLow          = parseField      tryU64       "TimeLow"          "Could not parse TimeLow"
-let getTimeHigh         = parseOptField   tryU64       "TimeHigh"
-let getAuditPath        = parseAuditPath               "AuditPath"        "Could not parse AuditPath"
-let getValue            = parseField      tryU64       "Value"            "Could not parse Value"
-let getCWT              = parseField      tryString    "CWT"              "Could not parse CWT"
-let getDefaultHash      = parseField      tryHash      "DefaultHash"      "Could not parse DefaultHash"
-let getPosition         = parsePosition                "Position"         "Could not parse Position"
-let getOracleContractId = parseContractId              "OracleContractId" "Could not parse OracleContractId"
+val getTimestamp        : parser U64.t          82
+val getCommit           : parser hash           82
+val getOraclePubKey     : parser publicKey      82
+val getTicker           : parser ticker         94
+val getPriceLow         : parser U64.t          82
+val getPriceHigh        : parser (option U64.t) 77
+val getTimeLow          : parser U64.t          82
+val getTimeHigh         : parser (option U64.t) 77
+val getAuditPath        : parser auditPath      5764
+val getValue            : parser U64.t          82
+val getCWT              : parser string         82
+val getDefaultHash      : parser hash           82
+val getPosition         : parser position       91
+val getOracleContractId : parser contractId     162
 
-val parseProof: option (Dict.t data) -> result proof `cost` 910
-let parseProof dict =
+let getTimestamp        dict = dict |>
+    parseField      tryU64       "Timestamp"        "Could not parse Timestamp"
+let getCommit           dict = dict |>
+    parseField      tryHash      "Commit"           "Could not parse Commit"
+let getOraclePubKey     dict = dict |>
+    parseField      tryPublicKey "OraclePubKey"     "Could not parse OraclePubKey"
+let getTicker           dict = dict |>
+    parseTicker                  "Ticker"           "Could not parse Ticker"
+let getPriceLow         dict = dict |>
+    parseField      tryU64       "PriceLow"         "Could not parse PriceLow"
+let getPriceHigh        dict = dict |>
+    parseOptField   tryU64       "PriceHigh"
+let getTimeLow          dict = dict |>
+    parseField      tryU64       "TimeLow"          "Could not parse TimeLow"
+let getTimeHigh         dict = dict |>
+    parseOptField   tryU64       "TimeHigh"
+let getAuditPath        dict = dict |>
+    parseAuditPath               "AuditPath"        "Could not parse AuditPath"
+let getValue            dict = dict |>
+    parseField      tryU64       "Value"            "Could not parse Value"
+let getCWT              dict = dict |>
+    parseField      tryString    "CWT"              "Could not parse CWT"
+let getDefaultHash      dict = dict |>
+    parseField      tryHash      "DefaultHash"      "Could not parse DefaultHash"
+let getPosition         dict = dict |>
+    parsePosition                "Position"         "Could not parse Position"
+let getOracleContractId dict = dict |>
+    parseContractId              "OracleContractId" "Could not parse OracleContractId"
+
+val parseProof: option (Dict.t data) -> result proof `cost` 6217
+let parseProof dict = // 31
     let open RT in
-    dict |> getTicker      >>= (fun key         ->
-    dict |> getValue       >>= (fun value       ->
-    dict |> getCommit      >>= (fun root        ->
-    dict |> getAuditPath   >>= (fun auditPath   ->
-    dict |> getCWT         >>= (fun cwt         ->
-    dict |> getDefaultHash >>= (fun defaultHash ->
+    dict |> getTicker      >>= (fun key         -> // 94
+    dict |> getValue       >>= (fun value       -> // 82
+    dict |> getCommit      >>= (fun root        -> // 82
+    dict |> getAuditPath   >>= (fun auditPath   -> // 5764
+    dict |> getCWT         >>= (fun cwt         -> // 82
+    dict |> getDefaultHash >>= (fun defaultHash -> // 82
         RT.ok ({
             key         = key;
             value       = value;
@@ -276,28 +320,28 @@ let parseProof dict =
             defaultHash = defaultHash;
         })))))))
 
-val parseAttestation: option (Dict.t data) -> result attestation `cost` 198
-let parseAttestation dict =
+val parseAttestation: option (Dict.t data) -> result attestation `cost` 262
+let parseAttestation dict = // 16
     let open RT in
-    dict |> getTimestamp    >>= (fun timestamp ->
-    dict |> getCommit       >>= (fun commit    ->
-    dict |> getOraclePubKey >>= (fun pubKey    ->
+    dict |> getTimestamp    >>= (fun timestamp -> // 82
+    dict |> getCommit       >>= (fun commit    -> // 82
+    dict |> getOraclePubKey >>= (fun pubKey    -> // 82
         RT.ok ({
             timestamp = timestamp;
             commit    = commit;
             pubKey    = pubKey;
         }))))
 
-val parseEvent: option (Dict.t data) -> result event `cost` 526
-let parseEvent dict =
+val parseEvent: option (Dict.t data) -> result event `cost` 692
+let parseEvent dict = // 36
     let open RT in
-    dict |> getOraclePubKey     >>= (fun oraclePubKey     ->
-    dict |> getOracleContractId >>= (fun oracleContractId ->
-    dict |> getTicker           >>= (fun ticker           ->
-    dict |> getPriceLow         >>= (fun priceLow         ->
-    dict |> getPriceHigh        >>= (fun priceHigh        ->
-    dict |> getTimeLow          >>= (fun timeLow          ->
-    dict |> getTimeHigh         >>= (fun timeHigh         ->
+    dict |> getOraclePubKey     >>= (fun oraclePubKey     -> // 82
+    dict |> getOracleContractId >>= (fun oracleContractId -> // 162
+    dict |> getTicker           >>= (fun ticker           -> // 94
+    dict |> getPriceLow         >>= (fun priceLow         -> // 82
+    dict |> getPriceHigh        >>= (fun priceHigh        -> // 77
+    dict |> getTimeLow          >>= (fun timeLow          -> // 82
+    dict |> getTimeHigh         >>= (fun timeHigh         -> // 77
         RT.ok ({
             oraclePubKey     = oraclePubKey;
             oracleContractId = oracleContractId;
@@ -308,13 +352,13 @@ let parseEvent dict =
             timeHigh         = timeHigh;
         }))))))))
 
-val parseRedemption: option (Dict.t data) -> result redemption `cost` 1700
-let parseRedemption dict =
+val parseRedemption: option (Dict.t data) -> result redemption `cost` 7284
+let parseRedemption dict = // 22
     let open RT in
-    dict |> parseEvent       >>= (fun event       ->
-    dict |> getPosition      >>= (fun position    ->
-    dict |> parseAttestation >>= (fun attestation ->
-    dict |> parseProof       >>= (fun proof       ->
+    dict |> parseEvent       >>= (fun event       -> // 692
+    dict |> getPosition      >>= (fun position    -> // 91
+    dict |> parseAttestation >>= (fun attestation -> // 262
+    dict |> parseProof       >>= (fun proof       -> // 6217
         RT.ok ({
             bet         = {
                 event    = event;
@@ -332,64 +376,74 @@ let parseRedemption dict =
 -------------------------------------------------------------------------------
 *)
 
-let updatePublicKey (pk:publicKey) (s:Sha3.t): Sha3.t `cost` 330 =
-    let! cpk = compress pk in
+val updatePublicKey : hashUpdate publicKey 517
+let updatePublicKey pk s = // 7
+    let! cpk = compress pk in // 305
     ret s
-    >>= updateCPK cpk
+    >>= updateCPK cpk // 205
 
 // Sha3.updateString with a constant cost
-let updateTicker (tick:ticker) (s:Sha3.t): Sha3.t `cost` 24 =
+val updateTicker : hashUpdate ticker 36
+let updateTicker tick s = // 12
     ret s
-    >>= Sha3.updateString tick
+    >>= Sha3.updateString tick // (6 * Str.length tick)
     >>= incRet (6 * (4 - Str.length tick))
 
-let updateContractId ((v,h):contractId) (s:Sha3.t): Sha3.t `cost` 216 =
+val updateContractId : hashUpdate contractId 223
+let updateContractId (v,h) s = // 7
     ret s
-    >>= Sha3.updateU32 v
-    >>= Sha3.updateHash h
+    >>= Sha3.updateU32  v // 24
+    >>= Sha3.updateHash h // 192
 
-let updateEvent (event:event) (s:Sha3.t): Sha3.t `cost` 762 =
+val updateEvent : hashUpdate event 1009
+let updateEvent event s = // 31
     ret s
-    >>= updatePublicKey         event.oraclePubKey
-    >>= updateContractId        event.oracleContractId
-    >>= updateTicker            event.ticker
-    >>= Sha3.updateU64          event.priceLow
-    >>= Sha3.updateU64 `runOpt` event.priceHigh
-    >>= Sha3.updateU64          event.timeLow
-    >>= Sha3.updateU64 `runOpt` event.timeHigh
+    >>= updatePublicKey         event.oraclePubKey     // 517
+    >>= updateContractId        event.oracleContractId // 223
+    >>= updateTicker            event.ticker           // 36
+    >>= Sha3.updateU64          event.priceLow         // 48
+    >>= Sha3.updateU64 `runOpt` event.priceHigh        // 53
+    >>= Sha3.updateU64          event.timeLow          // 48
+    >>= Sha3.updateU64 `runOpt` event.timeHigh         // 53
 
-let updatePosition (position:position) (s:Sha3.t): Sha3.t `cost` 24 =
+val updatePosition : hashUpdate position 30
+let updatePosition position s = // 6
     ret s
-    >>= Sha3.updateString
+    >>= Sha3.updateString // 24
     begin match position with
     | Bull -> "Bull"
     | Bear -> "Bear"
     end
 
-let hashCommitment (attestation:attestation): hash `cost` 590 =
+val hashCommitment : attestation -> hash `cost` 792
+let hashCommitment attestation = // 15
     ret Sha3.empty
-    >>= Sha3.updateHash attestation.commit
-    >>= Sha3.updateU64  attestation.timestamp
-    >>= updatePublicKey attestation.pubKey
-    >>= Sha3.finalize
+    >>= Sha3.updateHash attestation.commit    // 192
+    >>= Sha3.updateU64  attestation.timestamp // 48
+    >>= updatePublicKey attestation.pubKey    // 517
+    >>= Sha3.finalize                         // 20
 
-let hashAttestation (attestation:attestation): hash `cost` 802 =
-    let! commit = hashCommitment attestation in
+val hashAttestation : attestation -> hash `cost` 1013
+let hashAttestation attestation = // 9
+    let! commit = hashCommitment attestation in // 792
     ret Sha3.empty
-    >>= Sha3.updateHash commit
-    >>= Sha3.finalize
+    >>= Sha3.updateHash commit // 192
+    >>= Sha3.finalize          // 20
 
-let hashBet (bet:bet): hash `cost` 806 =
+val hashBet : bet -> hash `cost` 1070
+let hashBet bet = // 11
     ret Sha3.empty
-    >>= updateEvent    bet.event
-    >>= updatePosition bet.position
-    >>= Sha3.finalize
+    >>= updateEvent    bet.event    // 1009
+    >>= updatePosition bet.position // 30
+    >>= Sha3.finalize               // 20
 
-let mkBetToken ((v, h):contractId) (bet:bet): asset `cost` 806 =
+val mkBetToken : contractId -> bet -> asset `cost` 1077
+let mkBetToken (v, h) bet = // 7
     let! betHash = hashBet bet in
     ret (v, h, betHash)
 
-let mkAttestToken ((v,h):contractId) (attestation:attestation): asset `cost` 802 =
+val mkAttestToken : contractId -> attestation -> asset `cost` 1020
+let mkAttestToken (v,h) attestation = // 7
     let! attestHash = hashAttestation attestation in
     ret (v, h, attestHash)
 
@@ -401,29 +455,29 @@ let mkAttestToken ((v,h):contractId) (attestation:attestation): asset `cost` 802
 -------------------------------------------------------------------------------
 *)
 
-val inBounds : U64.t -> option U64.t -> U64.t -> bool `cost` 0
+val inBounds : U64.t -> option U64.t -> U64.t -> bool `cost` 10
 let inBounds low high value =
     (low `U64.lte` value && Opt.maybe true (U64.lte value) high)
     |> ret
 
-val validateTime: redemption -> result redemption `cost` 0
-let validateTime redemption =
+val validateTime: redemption -> result redemption `cost` 25
+let validateTime redemption = // 15
     let  event = redemption.bet.event             in
     let  low   = event.timeLow                    in
     let  high  = event.timeHigh                   in
     let  value = redemption.attestation.timestamp in
-    let! inb   = inBounds low high value          in
+    let! inb   = inBounds low high value          in // 10
     if inb
         then RT.ok redemption
         else RT.failw "Attestation time is not within the given time bounds"
 
-val validatePrice: redemption -> result redemption `cost` 0
-let validatePrice redemption =
+val validatePrice: redemption -> result redemption `cost` 31
+let validatePrice redemption = // 21
     let  event = redemption.bet.event    in
     let  low   = event.priceLow          in
     let  high  = event.priceHigh         in
     let  value = redemption.proof.value  in
-    let! inb   = inBounds low high value in
+    let! inb   = inBounds low high value in // 10
     let  pos   = redemption.bet.position in
     match inb, pos with
     | true , Bull
@@ -432,31 +486,33 @@ let validatePrice redemption =
     | _ ->
         RT.failw "Position doesn't match the event"
 
-val hashKey : ticker -> hash `cost` 44
-let hashKey s =
-    Sha3.ofString s
-    |> inc (24 - (6 * Str.length s))
+val hashKey : ticker -> hash `cost` 53
+let hashKey s = // 9
+    Sha3.ofString s // (6 * (Str.length s) + 20)
+    |> inc (24 - (6 * Str.length s)) // 44
 
-val verifyAuditPath : proof -> bool `cost` 107568
-let verifyAuditPath proof =
-    let! key   = hashKey proof.key            in
+val verifyAuditPath : proof -> bool `cost` 107594
+let verifyAuditPath proof = // 17
+    let! key   = hashKey proof.key            in // 53
     let  value = SMT.serializeU64 proof.value in
-    SMT.verify proof.cwt proof.defaultHash proof.root proof.auditPath key (Some value)
+    SMT.verify proof.cwt proof.defaultHash proof.root proof.auditPath key (Some value) // 107524
 
-val validateAuditPath: redemption -> result redemption `cost` 107568
-let validateAuditPath redemption =
-    let! b = verifyAuditPath redemption.proof in
+val validateAuditPath: redemption -> result redemption `cost` 107602
+let validateAuditPath redemption = // 8
+    let! b = verifyAuditPath redemption.proof in // 107594
     if b
         then RT.ok redemption
         else RT.failw "Invalid audit path"
 
-val validateRedemption: redemption -> result redemption `cost` 107568
-let validateRedemption =
+val validateRedemption: redemption -> result redemption `cost` 107665
+let validateRedemption redemption = // 7
     let open RT in
-    ret
-    >=> validateTime
-    >=> validatePrice
-    >=> validateAuditPath
+    ret redemption
+    >>= validateTime      // 25
+    >>= validatePrice     // 31
+    >>= validateAuditPath // 107602
+
+
 
 (*
 -------------------------------------------------------------------------------
@@ -464,25 +520,25 @@ let validateRedemption =
 -------------------------------------------------------------------------------
 *)
 
-val buyEvent: txSkeleton -> contractId -> sender -> event -> CR.t `cost` 2635
-let buyEvent txSkel contractId sender event =
-    let! bullToken = mkBetToken contractId ({event=event; position=Bull}) in
-    let! bearToken = mkBetToken contractId ({event=event; position=Bear}) in
-    let! m         = TX.getAvailableTokens Asset.zenAsset txSkel          in
+val buyEvent: txSkeleton -> contractId -> sender -> event -> CR.t `cost` 3632
+let buyEvent txSkel contractId sender event = // 37
+    let! bullToken = mkBetToken contractId ({ event=event; position=Bull }) in // 1077
+    let! bearToken = mkBetToken contractId ({ event=event; position=Bear }) in // 1077
+    let! m         = TX.getAvailableTokens Asset.zenAsset txSkel            in // 64
     ret txSkel
-    >>= TX.mint m bullToken
-    >>= TX.mint m bearToken
-    >>= lockToSender bullToken m sender
-    >>= lockToSender bearToken m sender
-    >>= CR.ofTxSkel
+    >>= TX.mint m bullToken             // 64
+    >>= TX.mint m bearToken             // 64
+    >>= lockToSender bullToken m sender // 623
+    >>= lockToSender bearToken m sender // 623
+    >>= CR.ofTxSkel                     // 3
 
-val buy: txSkeleton -> contractId -> sender -> option data -> CR.t `cost` 3165
-let buy txSkel contractId sender =
+val buy: txSkeleton -> contractId -> sender -> option data -> CR.t `cost` 4349
+let buy txSkel contractId sender dict = // 10
     let open RT in
-    ret
-    >=> parseDict
-    >=> parseEvent
-    >=> buyEvent txSkel contractId sender
+    ret dict
+    >>= parseDict                         // 15
+    >>= parseEvent                        // 692
+    >>= buyEvent txSkel contractId sender // 3632
 
 
 
@@ -492,27 +548,29 @@ let buy txSkel contractId sender =
 -------------------------------------------------------------------------------
 *)
 
-val redeemRedemption: txSkeleton -> contractId -> sender -> redemption -> CR.t `cost` 2217
-let redeemRedemption txSkel contractId sender redemption =
-    let! betToken         = mkBetToken contractId redemption.bet       in
+val redeemRedemption: txSkeleton -> contractId -> sender -> redemption -> CR.t `cost` 2948
+let redeemRedemption txSkel contractId sender redemption = // 33
+    let! betToken         = mkBetToken contractId redemption.bet       in // 1077
     let  oracleContractId = redemption.bet.event.oracleContractId      in
     let  attestation      = redemption.attestation                     in
-    let! attestToken      = mkAttestToken oracleContractId attestation in
-    let! m                = TX.getAvailableTokens betToken txSkel      in
+    let! attestToken      = mkAttestToken oracleContractId attestation in // 1020
+    let! m                = TX.getAvailableTokens betToken txSkel      in // 64
     ret txSkel
-    >>= TX.destroy m betToken
-    >>= TX.destroy 1UL attestToken
-    >>= lockToSender Asset.zenAsset m sender
-    >>= CR.ofTxSkel
+    >>= TX.destroy m betToken                // 64
+    >>= TX.destroy 1UL attestToken           // 64
+    >>= lockToSender Asset.zenAsset m sender // 623
+    >>= CR.ofTxSkel                          // 3
 
-val redeem: txSkeleton -> contractId -> sender -> option data -> CR.t `cost` 111489
-let redeem txSkel contractId sender =
+val redeem: txSkeleton -> contractId -> sender -> option data -> CR.t `cost` 117924
+let redeem txSkel contractId sender dict = // 12
     let open RT in
-    ret
-    >=> parseDict
-    >=> parseRedemption
-    >=> validateRedemption
-    >=> redeemRedemption txSkel contractId sender
+    ret dict
+    >>= parseDict                                 // 15
+    >>= parseRedemption                           // 7284
+    >>= validateRedemption                        // 107665
+    >>= redeemRedemption txSkel contractId sender // 2948
+
+
 
 (*
 -------------------------------------------------------------------------------
@@ -529,14 +587,26 @@ val main:
     -> messageBody : option data
     -> wallet      : wallet
     -> state       : option data
-    -> CR.t `cost` 111489
-let main txSkel context contractId command sender messageBody wallet state =
+    -> CR.t `cost` 117934
+let main txSkel context contractId command sender messageBody wallet state = // 10
     match command with
     | "Buy" ->
-        buy txSkel contractId sender messageBody
-        |> inc 108324
+        buy txSkel contractId sender messageBody // 4349
+        |> inc 113575
     | "Redeem" ->
-        redeem txSkel contractId sender messageBody
+        redeem txSkel contractId sender messageBody // 117924
     | _ ->
         RT.failw "Unsupported command"
-        |> inc 111489
+        |> inc 117924
+
+val cf:
+       txSkel     : txSkeleton
+    -> context    : context
+    -> command    : string
+    -> sender     : sender
+    -> messageBody: option data
+    -> wallet     : wallet
+    -> state      : option data
+    -> nat `cost` 2
+let cf _ _ _ _ _ _ _ =
+    (117934 <: nat) |> ret
